More specs for LowStar.Permissions and draft for LowStar.Permissions.Pointer

ulib/LowStar.Permissions.Pointer.fst
@@ -9,34 +9,32 @@ open LowStar.Resource
 open LowStar.RST
 
 open LowStar.BufferOps
-open FStar.Permissions
+open LowStar.Permissions
+open FStar.Real
 
-private noeq type pointer (a: Type0) = {
-  v: B.pointer (a & Ghost.erased (value_perms a));
-  pid: Ghost.erased pos
+type value_with_perms (a: Type0) = vp : (a & Ghost.erased (value_perms a)){
+  let (v, p) = vp in
+  forall (pid:live_pid (Ghost.reveal p)). get_snapshot_from_pid (Ghost.reveal p) pid == v
 }
 
-private noeq type pointer_view (a: Type0) = {
-  view_v: a;
-  view_perm_kind: Ghost.erased permission_kind
+noeq type pointer (a: Type0) (perm: permission_kind) = {
+  v: B.pointer (value_with_perms a);
+  pid: Ghost.erased perm_id
 }
 
-abstract
-let ptr_view (#a:Type) (ptr:pointer a) : view (pointer_view a) = 
+let ptr_view (#a:Type) (#perm: permission_kind) (ptr:pointer a perm) : view a = 
   reveal_view ();
   let fp = Ghost.hide (B.loc_addr_of_buffer ptr.v) in 
   let inv h = 
     let (_, perm_map) = Seq.index (B.as_seq h ptr.v) 0 in
-    B.live h ptr.v /\ B.freeable ptr.v /\ is_live_pid (Ghost.reveal perm_map) ptr.pid 
+    B.live h ptr.v /\ B.freeable ptr.v /\
+    get_perm_kind_from_pid (Ghost.reveal perm_map) (Ghost.reveal ptr.pid) = perm
   in
   let sel h = 
     let (_, perm_map) = Seq.index (B.as_seq h ptr.v) 0 in
     let perm = get_permission_from_pid (Ghost.reveal perm_map) (Ghost.reveal ptr.pid) in
     let snapshot = get_snapshot_from_pid (Ghost.reveal perm_map) (Ghost.reveal ptr.pid) in
-    { 
-      view_v = snapshot;
-      view_perm_kind = Ghost.hide (get_perm_kind_from_pid (Ghost.reveal perm_map) (Ghost.reveal ptr.pid))
-    }
+    snapshot
   in
   {
     fp = fp;
@@ -44,23 +42,20 @@ let ptr_view (#a:Type) (ptr:pointer a) : view (pointer_view a) =
     sel = sel
   }
 
-let ptr_resource (#a:Type) (ptr:pointer a) = 
+let ptr_resource (#a:Type) (#perm: permission_kind) (ptr:pointer a perm) = 
   as_resource (ptr_view ptr)
-
-let get_perm_kind (#a:Type) (ptr: pointer a) h0 : GTot permission_kind =
-  Ghost.reveal (sel (ptr_view ptr) h0).view_perm_kind
 
 let ptr_read 
   (#a: Type)
-  (ptr: pointer a)
+  (#perm: permission_kind)
+  (ptr: pointer a perm)
   : RST a 
     (ptr_resource ptr)
     (fun _ -> ptr_resource ptr)
-    (fun h0 -> allows_read (get_perm_kind ptr h0))
+    (fun _ -> allows_read perm)
     (fun h0 x h1 -> 
-      let view0 = sel (ptr_view ptr) h0 in 
-      let view1 = sel (ptr_view ptr) h1 in 
-      view0 == view1 /\ view0.view_v == x
+      x == sel (ptr_view ptr) h0 /\ 
+      sel (ptr_view ptr) h0 == sel (ptr_view ptr) h1
     )
   = 
   let (x, _) = !* ptr.v in
@@ -68,30 +63,29 @@ let ptr_read
 
 let ptr_write 
   (#a: Type)
-  (ptr: pointer a)
+  (#perm: permission_kind)
+  (ptr: pointer a perm)
   (x: a)
   : RST unit 
     (ptr_resource ptr)
     (fun _ -> ptr_resource ptr)
-    (fun h0 -> allows_write (get_perm_kind ptr h0))
-    (fun h0 _ h1 -> (sel (ptr_view ptr) h1) == { sel (ptr_view ptr) h0 with view_v = x})
-   =
-   reveal_rst_inv ();
-   reveal_modifies ();
-   let (_, perm_map) = !* ptr.v in
-   ptr.v *= (x, perm_map)
+    (fun _ -> allows_write perm)
+    (fun h0 _ h1 -> sel (ptr_view ptr) h1 == x)
+  =
+  reveal_rst_inv ();
+  reveal_modifies ();
+  let (_, perm_map) = !* ptr.v in
+  ptr.v *= (x, Ghost.hide (change_snapshot (Ghost.reveal perm_map) x))
 
-let ptr_alloc (#a:Type)
-              (init:a)
-            : RST (pointer a) (empty_resource)
-                                (fun ptr -> ptr_resource ptr)
-                                (fun _ -> True)
-                                (fun _ ptr h1 -> 
-                                   sel (ptr_view ptr) h1 == {
-                                     view_v = init; 
-                                     view_perm_kind = Ghost.hide FULL
-                                    }
-                                ) =
+let ptr_alloc 
+  (#a:Type)
+  (init:a)
+  : RST (pointer a FULL)
+    (empty_resource)
+    (fun ptr -> ptr_resource ptr)
+    (fun _ -> True)
+    (fun _ ptr h1 -> sel (ptr_view ptr) h1 == init)
+  =
   reveal_rst_inv ();
   reveal_modifies ();
   let perm_map = Ghost.hide (new_value_perms init) in
@@ -99,27 +93,46 @@ let ptr_alloc (#a:Type)
   let ptr_v = B.malloc HS.root (init, perm_map) 1ul in
   { v = ptr_v; pid = pid }
 
-let ptr_free (#a:Type)
-             (ptr:pointer a)
-           : RST unit (ptr_resource ptr)
-                      (fun ptr -> empty_resource)
-                      (fun h0 -> get_perm_kind ptr h0 = RW )
-                      (fun _ _ _ -> True) =
+let ptr_free
+  (#a:Type)
+  (ptr:pointer a FULL)
+  : RST unit
+    (ptr_resource ptr)
+    (fun ptr -> empty_resource)
+    (fun _ -> True )
+    (fun _ _ _ -> True)
+  =
   reveal_rst_inv ();
   reveal_modifies ();
   reveal_empty_resource ();
   B.free ptr.v
 
-let foo () : RST unit 
+#reset-options
+
+let read_write_without_sharing () : RST unit 
   (empty_resource)
   (fun _ -> empty_resource)
   (fun _ -> True)
   (fun _ _ _ -> True)
   = 
-  let ptr = ptr_alloc 42ul in
-  let x1 = ptr_read ptr in
-  ptr_write ptr FStar.UInt32.(x1 +^ 1ul);
-  ptr_free ptr;
-  //let x2 = ptr_read ptr in
+  let ptr = rst_frame 
+    (empty_resource)
+    (fun ptr -> ptr_resource ptr)
+    (fun _ -> ptr_alloc 42ul)
+  in
+  let x1 = rst_frame 
+    (ptr_resource ptr)
+    (fun _ -> ptr_resource ptr)
+    (fun _ -> ptr_read ptr)
+  in
+  rst_frame
+    (ptr_resource ptr)
+    (fun _ -> ptr_resource ptr)
+    (fun _ -> ptr_write ptr FStar.UInt32.(x1 +%^ 1ul));
+  rst_frame
+    (ptr_resource ptr) 
+    (fun _ -> empty_resource)
+    (fun _ -> ptr_free ptr);
   ()
+
 
